PDDL_to_STRIPS.thy
@@ -4,111 +4,413 @@ theory PDDL_to_STRIPS
     "Verified_SAT_Based_AI_Planning.STRIPS_Semantics"
     PDDL_Sema_Supplement Normalization_Definitions
     Utils Formula_Utils (* String_Shenanigans *)
+    "Propositional_Proof_Systems.CNF"
+    (* list linorder: *) "HOL-Library.List_Lexorder" "HOL-Library.Char_ord" (* only used to minimize negative variables *)
 begin
 
+term "sorted_list_of_set :: string set \<Rightarrow> string list"
 
-(* utils *)
-fun map_filter :: "('a \<rightharpoonup> 'b) \<Rightarrow> 'a list \<Rightarrow> 'b list" where
-  "map_filter f [] = []" |
-  "map_filter f (x # xs) = (case f x of None \<Rightarrow> map_filter f xs |
-    Some y \<Rightarrow> y # map_filter f xs)"
+text \<open>There are two big differences between normalized ground PDDL and
+  STRIPS. Normalized PDDL formulas are pure conjunctions, but they can contain
+  \<bottom> and negative atoms. These differences require workarounds:
+- We introduce negative variants of all ground predicates in the STRIPS task.
+  Init and operator effects are modified accordingly.
+  TODO: only use negative variables where needed, i.e.: when the goal clause or
+  operator preconditions contain the negative literal.
+- A new static variable that is always false is introduced to be used in place of \<bottom>.
+  Although technically not needed since it can always be removed from clauses,
+  we also introduce a static variable for \<not>\<bottom>.
+- Of course, we could also omit any operators whose preconditions contain \<bottom>, but this
+  seemed easier.
+\<close>
+
+(* converting conj into a clause as list *)
+(* assumes is_conj. TODO Utils *)
+fun as_clause :: "'a formula \<Rightarrow> 'a formula list" where
+  "as_clause (A \<^bold>\<and> B) = A # as_clause B" |
+  "as_clause A = [A]"
+
+definition "v\<^sub>T \<equiv> ''+'' :: name"
+definition "v\<^sub>F \<equiv> ''-'' :: name"
+abbreviation "vpos p \<equiv> CHR ''+'' # predicate.name p"
+abbreviation "vneg p \<equiv> CHR ''-'' # predicate.name p"
+lemmas vb_defs = v\<^sub>T_def v\<^sub>F_def
+
+fun pred_vpos :: "predicate_decl \<Rightarrow> name" where
+  "pred_vpos (PredDecl n args) = vpos n"
+fun pred_vneg :: "predicate_decl \<Rightarrow> name" where
+  "pred_vneg (PredDecl n args) = vneg n"
+
+(* Converting formulas into variables *)
+(* assumes is_lit_plus and not Eq *)
+fun lit_as_var :: "'a atom formula \<Rightarrow> name" where
+  "lit_as_var \<bottom> = v\<^sub>F" |
+  "lit_as_var (\<^bold>\<not>\<bottom>) = v\<^sub>T" |
+  "lit_as_var (Atom (predAtm n args)) = vpos n" |
+  "lit_as_var (\<^bold>\<not>(Atom (predAtm n args))) = vneg n"
+
+definition fmla_as_vars :: "'a atom formula \<Rightarrow> name list" where
+  "fmla_as_vars F \<equiv> map lit_as_var (as_clause F)"
+
+fun lit_as_goal :: "'a atom formula \<Rightarrow> (name \<times> bool)" where
+  "lit_as_goal \<bottom> = (v\<^sub>F, True)" |
+  "lit_as_goal (\<^bold>\<not>\<bottom>) = (v\<^sub>T, True)" | (* equivalent: (v\<^sub>F, False) *)
+  "lit_as_goal (Atom (predAtm n args)) = (vpos n, True)" |
+  "lit_as_goal (\<^bold>\<not>(Atom (predAtm n args))) = (vpos n, False)"
+
+abbreviation "fmla_as_goals F \<equiv> map lit_as_goal (as_clause F)"
+
+(* atm_as_vpos is technically subsumed by lit_as_var *)
+fun atm_as_vpos :: "'a atom formula \<Rightarrow> name" where
+  "atm_as_vpos (Atom (predAtm n args)) = vpos n"
+fun atm_as_vneg :: "'a atom formula \<Rightarrow> name" where
+  "atm_as_vneg (Atom (predAtm n args)) = vneg n"
+
+(* add effects take precedence *)
+(* removes duplicates *)
+fun fix_effect :: "'a ast_effect \<Rightarrow> 'a ast_effect" where
+  "fix_effect (Effect add del) = Effect add (filter (\<lambda>x. x \<notin> set add) del)"
+
+fun as_strips_op :: "ast_action_schema \<Rightarrow> name strips_operator" where
+  "as_strips_op (Action_Schema n args pre eff) =
+  (let eff' = fix_effect eff; add = adds eff'; del = dels eff' in
+  \<lparr>
+    precondition_of = fmla_as_vars pre
+    , add_effects_of = map atm_as_vpos add @ map atm_as_vneg del
+    , delete_effects_of = map atm_as_vpos del @ map atm_as_vneg add \<rparr>)"
 
 context ast_problem begin
 
-fun as_strips_var_p :: "predicate_decl \<Rightarrow> name" where
-  "as_strips_var_p (PredDecl (Pred n) args) = CHR ''+'' # n"
-fun as_strips_var_n :: "predicate_decl \<Rightarrow> name" where
-  "as_strips_var_n (PredDecl (Pred n) args) = CHR ''-'' # n"
-term Option.bind
+definition "pos_vars = v\<^sub>T # map pred_vpos (predicates D)"
+definition "neg_vars = v\<^sub>F # map pred_vneg (predicates D)"
+abbreviation "strips_vars \<equiv> pos_vars @ neg_vars"
+lemmas vars_defs = pos_vars_def neg_vars_def
+(*
+  initD: ["A", "B"]
+  pvars: + A B C,
+  nvars: - a b c,
+  "init": [+, A, B]
+  empty: +:0, A:0, B:0, C:0, -:1, a:1, b:1, c:1
+  init: +:1, A:1, B:1, C:0, -:0, a:0, b:0, c:1
+*)
 
-(* expects input to satisfy \<open>is_predAtom\<close> *)
-fun as_strips_atom_p :: "'a atom formula \<Rightarrow> name" where
-  "as_strips_atom_p (Atom (predAtm (Pred p) args)) = CHR ''+'' # p"
-fun as_strips_atom_n :: "'a atom formula \<Rightarrow> name" where
-  "as_strips_atom_n (Atom (predAtm (Pred p) args)) = CHR ''-'' # p"
+abbreviation "pos_empty \<equiv> fold (\<lambda>v s. s(v \<mapsto> False)) pos_vars (\<lambda>x. None)"
+definition "empty_state \<equiv> fold (\<lambda>v s. s(v \<mapsto> True)) neg_vars pos_empty"
+definition (in -) "upd_init a s \<equiv> s(atm_as_vpos a \<mapsto> True, atm_as_vneg a \<mapsto> False)"
+definition strips_init :: "name strips_state" where
+  "strips_init \<equiv> fold upd_init (init P) empty_state"
+lemmas init_defs = empty_state_def upd_init_def strips_init_def
 
-term is_conj
-term is_lit_plus
-(* todo, maybe use monads here? *)
-term omap
-fun (in -)option_Cons :: "'a option \<Rightarrow> 'a list option \<Rightarrow> 'a list option" where
-  "option_Cons _ None = None" |
-  "option_Cons None (Some xs) = None" |
-  "option_Cons (Some x) (Some xs) = Some (x # xs)"
-
-(*(* expects \<open>is_lit_plus\<close> but no Eq allowed *)
-fun as_strips_var :: "term atom formula \<rightharpoonup> name" where
-  "as_strips_pre \<bottom> = None" |
-  "as_strips_pre (\<^bold>\<not>\<bottom>) = Some []" |
-  "as_strips_pre (Atom a) = Some ([as_strips_atom_p (Atom a)])" *)
-
-(* expects \<open>is_conj p \<and> no_Eq p\<close> *)
-fun as_strips_pre :: "'a atom formula \<rightharpoonup> name list" where
-  "as_strips_pre \<bottom> = None" |
-  "as_strips_pre (\<^bold>\<not>\<bottom>) = Some []" |
-  "as_strips_pre (Atom a) = Some ([as_strips_atom_p (Atom a)])" |
-  "as_strips_pre (\<^bold>\<not>(Atom a)) = Some ([as_strips_atom_n (Atom a)])" |
-  "as_strips_pre (A \<^bold>\<and> B) = (case (as_strips_pre B) of None \<Rightarrow> None |
-    Some ys \<Rightarrow> (case (as_strips_pre A) of None \<Rightarrow> None |
-    Some y \<Rightarrow> Some (y @ ys)))"
-
-fun as_strips_op :: "ast_action_schema \<rightharpoonup> name strips_operator" where
-  "as_strips_op (Action_Schema n args pre (Effect add del)) =
-    (case as_strips_pre pre of None \<Rightarrow> None |
-    Some pre' \<Rightarrow> Some \<lparr>
-    precondition_of = pre'
-    , add_effects_of = map as_strips_atom_p add @ map as_strips_atom_n del
-    , delete_effects_of = map as_strips_atom_p del @ map as_strips_atom_n add \<rparr>)"
-
-term fold
-
-(* first set every variable to false *)
-(* then update those in init *)
-definition var_map :: "(name, bool) state" where
-  "var_map \<equiv>
-  (let ps = map as_strips_var_p (predicates D); ns = map as_strips_var_n (predicates D);
-    spos = fold (\<lambda>v c. c(v := Some False)) ps (\<lambda>x. None) in
-    fold (\<lambda>v c. c(v := Some True)) ns spos)"
-
-fun as_strips_init :: "(name, bool) state \<Rightarrow> 'a atom formula list \<Rightarrow> (name, bool) state" where
-  "as_strips_init c [] = c" |
-  "as_strips_init c (i # is) = (as_strips_init c is)(as_strips_atom_p i := Some True, as_strips_atom_n i := Some False)"
-
-(* expects \<open>is_conj p \<and> no_Eq p\<close> *)
-fun as_strips_goal :: "'a atom formula \<rightharpoonup> (name \<times> bool) list" where
-  "as_strips_goal \<bottom> = None" |
-  "as_strips_goal (\<^bold>\<not>\<bottom>) = Some []" |
-  "as_strips_goal (Atom a) = Some [(as_strips_atom_p (Atom a), True)]" |
-  "as_strips_goal (\<^bold>\<not>(Atom a)) = Some[(as_strips_atom_p (Atom a), False)]" |
-  "as_strips_goal (A \<^bold>\<and> B) = do {xs \<leftarrow> as_strips_goal A; ys \<leftarrow> as_strips_goal B; Some (xs @ ys)}"
-
-(* eliminate contradictions *)
-fun (in -) unique_mapof :: "(name \<times> bool) list \<rightharpoonup> (name, bool) state" where
-  "unique_mapof [] = Some (\<lambda>_. None)" |
-  "unique_mapof ((x, b) # xs) =
-    do {m \<leftarrow> unique_mapof xs; if m x = Some (\<not>b) then None else Some (m(x\<mapsto>b))}"
+fun (in -) upd_goal where "upd_goal (v, b) s = s(v \<mapsto> b)"
+definition strips_goal :: "name strips_state" where
+  "strips_goal \<equiv> fold upd_goal (fmla_as_goals (goal P)) (\<lambda>x. None)"
 
 definition as_strips :: "name strips_problem" where
   "as_strips \<equiv> \<lparr> 
-    variables_of = map as_strips_var_p (predicates D) @
-      map as_strips_var_n (predicates D)
-    , operators_of = map_filter as_strips_op (actions D)
-    , initial_of = as_strips_init var_map (init P)
-    , goal_of = the (unique_mapof (the (as_strips_goal (goal P)))) \<rparr>"
+    variables_of = strips_vars
+    , operators_of = map as_strips_op (actions D)
+    , initial_of = strips_init
+    , goal_of = strips_goal \<rparr>"
+
+definition "restore_pddl_pa op_i \<equiv> PAction (ac_name (actions D ! op_i)) []"
+definition "restore_pddl_plan op_is \<equiv> map restore_pddl_pa op_is"
 
 end
 
 lemmas to_strips_code =
-  ast_problem.as_strips_var_p.simps
-  ast_problem.as_strips_var_n.simps
-  ast_problem.as_strips_atom_p.simps
-  ast_problem.as_strips_atom_n.simps
-  ast_problem.as_strips_pre.simps
-  ast_problem.as_strips_op.simps
-  ast_problem.as_strips_init.simps
-  ast_problem.var_map_def
-  ast_problem.as_strips_goal.simps
+  ast_problem.vars_defs
+  ast_problem.init_defs
+  ast_problem.strips_goal_def
   ast_problem.as_strips_def
+  ast_problem.restore_pddl_pa_def
+  ast_problem.restore_pddl_plan_def
 declare to_strips_code[code]
+
+value "ast_problem.as_strips" (* checking if code exists *)
+
+subsection \<open> Alternative definitions \<close>
+
+context ast_problem begin
+
+lemma as_strips_op_sel:
+  fixes ac
+  defines "eff' \<equiv> fix_effect (ac_eff ac)"
+  shows "precondition_of (as_strips_op ac) = fmla_as_vars (ac_pre ac)"
+  "add_effects_of (as_strips_op ac) = map atm_as_vpos (adds eff') @ map atm_as_vneg (dels eff')"
+  "delete_effects_of (as_strips_op ac) = map atm_as_vpos (dels eff') @ map atm_as_vneg (adds eff')"
+  apply (cases ac) apply simp_all unfolding as_strips_op.simps Let_def apply simp
+  apply (cases ac) apply simp_all unfolding as_strips_op.simps Let_def eff'_def apply simp
+  apply (cases ac) apply simp_all unfolding as_strips_op.simps Let_def eff'_def by simp
+
+lemma as_strips_sel:
+  "as_strips \<^sub>\<V> = strips_vars"
+  "as_strips \<^sub>\<O> = map as_strips_op (actions D)"
+  "as_strips \<^sub>I = strips_init"
+  "as_strips \<^sub>G = strips_goal"
+  unfolding as_strips_def by simp_all
+end
+
+subsection \<open> Formula proofs \<close>
+
+(* TODO Utils *)
+lemma as_clause_sem: "A \<Turnstile> F \<longleftrightarrow> (\<forall>a \<in> set (as_clause F). A \<Turnstile> a)"
+  by (induction F) simp_all
+(* ? *)
+lemma as_clause_lits: assumes "is_conj F" shows "list_all1 is_lit_plus (as_clause F)"
+  using assms by (induction F rule: is_conj.induct) simp_all
+
+(* as_clause structure *)
+abbreviation (input) "no_eqs F \<equiv> \<forall>a b. Eq a b \<notin> atoms F"
+fun is_predatm_lit where
+  "is_predatm_lit \<bottom> = True" |
+  "is_predatm_lit (\<^bold>\<not>\<bottom>) = True" |
+  "is_predatm_lit (Atom (predAtm n args)) = True" |
+  "is_predatm_lit (\<^bold>\<not>(Atom (predAtm n args))) = True" |
+  "is_predatm_lit _ = False"
+(* ? *)
+lemma is_predatm_lit_plus: "is_predatm_lit F \<Longrightarrow> is_lit_plus F"
+  by (cases F rule: is_predatm_lit.cases) simp_all
+lemma no_eqs_as_clause:
+  assumes "is_conj F \<and> no_eqs F"
+  shows "list_all1 is_predatm_lit (as_clause F)"
+using assms proof (induction F rule: as_clause.induct)
+  case (1 A B)
+  thus ?case by (cases A rule: is_predatm_lit.cases) force+
+next
+  case ("2_1" a)
+  thus ?case by (cases a) simp_all
+next
+  case ("2_3" a)
+  thus ?case by (cases a rule: is_predAtom.cases) simp_all
+qed simp_all
+
+(* grounded no eq *)
+
+context wf_grounded_problem begin
+
+lemma objT_empty: "objT = (\<lambda>x. None)"
+  using grounded_prob grounded_dom
+  unfolding grounded_prob_def grounded_dom_def objT_def constT_def by auto
+
+lemma (in wf_ast_domain) wf_empty_atoms:
+  assumes "wf_fmla (\<lambda>x. None) F"
+  shows 
+    "\<forall>a \<in> atoms F. \<exists>n. a = predAtm n [] \<and> PredDecl n [] \<in> set (predicates D)"
+using assms proof (induction F)
+  case (Atom x)
+  then show ?case proof (cases x)
+    case (predAtm n args)
+    with Atom obtain Ts where 1: "sig n = Some Ts" "list_all2 (is_of_type (\<lambda>x. None)) args Ts"
+      unfolding predAtm wf_fmla.simps wf_atom.simps wf_pred_atom.simps
+      using case_optionE by blast
+    hence 2: "args = [] \<and> Ts = []" unfolding is_of_type_def
+      using list.rel_cases by auto
+    with 1 have "PredDecl n [] \<in> set (predicates D)"
+      using sig_Some by blast
+    with 2 show ?thesis using predAtm by simp
+  qed simp
+qed auto
+
+lemma (in wf_ast_domain) wf_empty_no_eqs:
+  assumes "wf_fmla (\<lambda>x. None) F"
+  shows "Eq a b \<notin> atoms F"
+  using assms wf_empty_atoms by blast
+
+lemma goal_no_eqs: "Eq a b \<notin> atoms (goal P)"
+  using objT_empty wf_P(5) wf_empty_no_eqs by simp
+
+context fixes ac assumes ac_in: "ac \<in> set (actions D)" begin
+
+lemma ac_tyt_empty: "ac_tyt ac = (\<lambda>x. None)"
+proof -
+  have 1: "constT = (\<lambda>x. None)" using grounded_dom grounded_dom_def constT_def by simp
+  from ac_in have "grounded_ac ac" using grounded_dom grounded_dom_def by blast
+  hence 2: "ac_params ac = []" by (cases ac) simp
+  thus "?thesis"
+    apply (intro ext)
+    subgoal for x
+      using 1 2 by (cases x) simp_all
+    done
+qed
+
+lemma pre_no_eqs: "Eq a b \<notin> atoms (ac_pre ac)"
+  using ac_in ac_tyt_empty
+  using wf_D(7) wf_action_schema_alt wf_empty_no_eqs  by metis
+
+lemma ac_pre_atoms:
+  "\<forall>a \<in> atoms (ac_pre ac). \<exists>n. a = predAtm n [] \<and> PredDecl n [] \<in> set (predicates D)"
+  using ac_in ac_tyt_empty
+  using wf_D(7) wf_action_schema_alt wf_empty_atoms by metis
+
+lemma ac_eff_empty:
+  "list_all1 (wf_fmla_atom (\<lambda>x. None)) (adds (ac_eff ac))"
+  "list_all1 (wf_fmla_atom (\<lambda>x. None)) (dels (ac_eff ac))"
+  using ac_in ac_tyt_empty
+  using wf_D(7) wf_action_schema_alt wf_effect_alt by metis+
+
+end
+
+(* not needed for init and effs, since it direcly follows with wf_fmla_atom_alt *)
+end
+
+subsection \<open> STRIPS task is WF \<close>
+
+context wf_normed_grounded_problem begin
+
+thm ListMem_iff
+
+thm wf_fmla_alt
+
+lemma a: "PredDecl n [] \<in> set (predicates D) \<Longrightarrow> vpos n \<in> pred_vpos ` set (predicates D)"
+  by force
+lemma b: "PredDecl n [] \<in> set (predicates D) \<Longrightarrow> vneg n \<in> pred_vneg ` set (predicates D)"
+  by force
+
+
+lemma fmla_vars_covered:
+  assumes "is_conj F" "\<forall>a \<in> atoms F. \<exists>n. a = predAtm n [] \<and> PredDecl n [] \<in> set (predicates D)"
+  shows "set (fmla_as_vars F) \<subseteq> set strips_vars"
+  unfolding fmla_as_vars_def vars_defs
+  using assms apply (induction F rule: as_clause.induct)
+  subgoal for A apply (cases A rule: lit_as_var.cases)
+    apply simp_all
+    using a b by fast+
+  subgoal for v by (cases v) force+
+  apply simp_all
+  subgoal for v by (cases v rule: is_predAtom.cases) force+
+  done
+
+thm wf_empty_atoms
+
+lemma wf_empty_fmla_atom:
+  assumes "wf_fmla_atom (\<lambda>x. None) a"
+  shows "\<exists>n. a = Atom (predAtm n []) \<and> PredDecl n [] \<in> set (predicates D)"
+  using assms wf_empty_atoms
+  unfolding wf_fmla_atom_alt
+  apply (cases a rule: is_predAtom.cases) by fastforce+
+
+lemma wf_empty_atom_covered:
+  assumes "wf_fmla_atom (\<lambda>x. None) a"
+  shows "atm_as_vpos a \<in> set strips_vars" "atm_as_vneg a \<in> set strips_vars"
+  unfolding vars_defs
+  using assms[THEN wf_empty_fmla_atom] apply (cases a rule: is_predAtom.cases) apply force+
+  using assms[THEN wf_empty_fmla_atom] apply (cases a rule: is_predAtom.cases) by force+
+
+find_theorems "set (map ?f ?xs) = ?f ` set ?xs"
+
+abbreviation "empty_atom a \<equiv> \<exists>n. a = Atom (predAtm n []) \<and> PredDecl n [] \<in> set (predicates D)"
+
+lemma wf_as_strips_op:
+  assumes "ac \<in> set (actions D)"
+  shows "is_valid_operator_strips as_strips (as_strips_op ac)"
+  unfolding is_valid_operator_strips_def Let_def ListMem_iff Ball_set[symmetric]
+  unfolding as_strips_sel
+  apply (intro conjI)
+  unfolding as_strips_op_sel
+proof -
+  from assms have "no_eqs (ac_pre ac)" using pre_no_eqs by blast
+  note 1 = ac_pre_atoms[OF assms]
+  from assms have "is_conj (ac_pre ac)"
+    using normed_dom unfolding prec_normed_dom_def by fast
+
+  from fmla_vars_covered[OF this 1] show "\<forall>v\<in>set (fmla_as_vars (ac_pre ac)). v \<in> set strips_vars"
+    by blast
+
+  obtain a d where eff: "ac_eff ac = Effect a d" by (cases "ac_eff ac") simp
+
+  have 1: "\<forall>v \<in> atm_as_vpos ` set a. v \<in> set strips_vars"
+          "\<forall>v \<in> atm_as_vneg ` set a. v \<in> set strips_vars"
+          "\<forall>v \<in> atm_as_vpos ` set d. v \<in> set strips_vars"
+          "\<forall>v \<in> atm_as_vneg ` set d. v \<in> set strips_vars"
+    using eff wf_empty_atom_covered ac_eff_empty[OF assms] by auto
+
+  thus "\<forall>v\<in>set (map atm_as_vpos (adds (fix_effect (ac_eff ac))) @
+             map atm_as_vneg (dels (fix_effect (ac_eff ac)))).
+       v \<in> set strips_vars" unfolding eff by auto
+
+  from 1 show "\<forall>v\<in>set (map atm_as_vpos (dels (fix_effect (ac_eff ac))) @
+             map atm_as_vneg (adds (fix_effect (ac_eff ac)))).
+       v \<in> set strips_vars" unfolding eff by auto
+
+  let ?adds = "adds (fix_effect (ac_eff ac))"
+  let ?dels = "dels (fix_effect (ac_eff ac))"
+
+  note ac_eff_empty[OF assms] wf_empty_fmla_atom
+  hence eatms: "list_all1 empty_atom ?adds \<and> list_all1 empty_atom ?dels"
+    by (cases "ac_eff ac") auto
+  have v_inj: "x \<noteq> y \<Longrightarrow> empty_atom x \<Longrightarrow> empty_atom y \<Longrightarrow>
+    atm_as_vpos x \<noteq> atm_as_vpos y \<and> atm_as_vneg x \<noteq> atm_as_vneg y" for x y
+    apply (cases x rule: is_predAtom.cases; cases y rule: is_predAtom.cases; simp)
+    subgoal for u v apply (cases u; cases v) by simp done
+  have p_neq_n: "empty_atom x \<Longrightarrow> atm_as_vpos x \<noteq> atm_as_vneg x" for x
+    by (cases x rule: is_predAtom.cases) simp_all
+
+  have 0: "set ?adds \<inter> set ?dels = {}"
+    by (cases "ac_eff ac") auto
+  have 1: "atm_as_vpos ` set ?adds \<inter> atm_as_vpos ` set ?dels = {}"
+  proof -
+    have "\<forall>x \<in> set ?adds. \<forall>y \<in> set ?dels. x \<noteq> y" using 0 by blast
+    hence "\<forall>x \<in> set ?adds. \<forall>y \<in> set ?dels. atm_as_vpos x \<noteq> atm_as_vpos y"
+      using eatms v_inj by metis
+    thus ?thesis by blast
+  qed
+  have 2: "atm_as_vneg ` set ?adds \<inter> atm_as_vneg ` set ?dels = {}"
+  proof -
+    have "\<forall>x \<in> set ?adds. \<forall>y \<in> set ?dels. x \<noteq> y" using 0 by blast
+    hence "\<forall>x \<in> set ?adds. \<forall>y \<in> set ?dels. atm_as_vneg x \<noteq> atm_as_vneg y"
+      using eatms v_inj by metis
+    thus ?thesis by blast
+  qed
+  have 3:
+    "atm_as_vpos ` set ?adds \<inter> atm_as_vneg ` set ?adds = {}"
+  proof -
+    {
+      fix x y assume a: "x \<in> set ?adds" "y \<in> set ?adds"
+      hence "empty_atom x" "empty_atom y" by (simp_all add: eatms)
+      hence "atm_as_vneg x \<noteq> atm_as_vpos y"
+        using eatms by (cases x rule: is_predAtom.cases; cases y rule: is_predAtom.cases)
+        simp_all
+    }
+    thus ?thesis by force
+  qed
+  have 4: "atm_as_vpos ` set ?dels \<inter> atm_as_vneg ` set ?dels = {}"
+  proof -
+    {
+      fix x y assume a: "x \<in> set ?dels" "y \<in> set ?dels"
+      hence "empty_atom x" "empty_atom y" by (simp_all add: eatms)
+      hence "atm_as_vneg x \<noteq> atm_as_vpos y"
+        using eatms by (cases x rule: is_predAtom.cases; cases y rule: is_predAtom.cases)
+        simp_all
+    }
+    thus ?thesis by force
+  qed
+
+  show "\<forall>v\<in>set (map atm_as_vpos (adds (fix_effect (ac_eff ac))) @
+             map atm_as_vneg (dels (fix_effect (ac_eff ac)))).
+       v \<notin> set (map atm_as_vpos (dels (fix_effect (ac_eff ac))) @
+                 map atm_as_vneg (adds (fix_effect (ac_eff ac))))"
+    apply simp
+    using 1 2 3 4
+    by (metis Set.set_insert Un_iff insert_disjoint(1))
+
+  show "\<forall>v\<in>set (map atm_as_vpos (dels (fix_effect (ac_eff ac))) @
+             map atm_as_vneg (adds (fix_effect (ac_eff ac)))).
+       v \<notin> set (map atm_as_vpos (adds (fix_effect (ac_eff ac))) @
+                 map atm_as_vneg (dels (fix_effect (ac_eff ac))))"
+    apply simp
+    using 1 2 3 4
+    by (metis Set.set_insert Un_iff insert_disjoint(1))
+qed
+
+theorem wf_as_strips: "is_valid_problem_strips as_strips"
+  unfolding is_valid_problem_strips_def Let_def as_strips_sel
+  apply (intro conjI)
+  using wf_as_strips_op unfolding Ball_set[symmetric] apply simp
+  oops
+
+
+
+
+end
 
 end
