Grounded_PDDL.thy
@@ -454,15 +454,6 @@ subsection \<open> Semantics \<close>
 
 text \<open> ground locale setup \<close>
 
-locale wf_grounded_domain = wf_ast_domain +
-  assumes grounded_dom: grounded_dom
-
-locale wf_grounded_problem = wf_ast_problem +
-  assumes grounded_prob: grounded_prob
-
-sublocale wf_grounded_problem \<subseteq> wf_grounded_domain D
-  using grounded_prob grounded_prob_def by (unfold_locales) simp
-
 sublocale wf_grounder \<subseteq> dg: wf_grounded_domain ground_dom
   using ground_dom_grounded
   by unfold_locales simp
@@ -471,27 +462,7 @@ sublocale wf_grounder \<subseteq> pg: wf_grounded_problem ground_prob
   using ground_prob_grounded
   by unfold_locales simp
 
-subsection \<open> Properties of grounded tasks \<close>
 
-lemma (in wf_grounded_problem) grounded_pa_nullary:
-  "wf_plan_action (PAction n args) \<longleftrightarrow> n \<in> ac_name ` set (actions D) \<and> args = []" (is "?L \<longleftrightarrow> ?R")
-proof -
-  have empty: "ac_params ac = []" if "ac \<in> set (actions D)" for ac
-    using that grounded_dom grounded_dom_def grounded_ac.simps
-    by (metis ast_action_schema.exhaust_sel that)
-  show ?thesis proof
-    assume ?L
-    then obtain ac where ac: "ac \<in> set (actions D)" "action_params_match ac args" "ac_name ac = n"
-      using wf_pa_refs_ac by metis
-    with ac show ?R using empty action_params_match_def by auto
-  next
-    assume ?R
-    then obtain ac where ac: "ac \<in> set (actions D)" "ac_name ac = n" by blast
-    with \<open>?R\<close> show ?L
-      unfolding wf_plan_action_simple action_params_match_def
-      using res_aux[of n ac] empty by simp
-  qed
-qed
 
 subsection \<open> Grounder Semantics \<close>
 
